Bitmap/Lemmas.lean
@@ -5,6 +5,7 @@ import Bitmap.Lemmas.Png.Adam7
 import Bitmap.Lemmas.Png.Gray1
 import Bitmap.Lemmas.Png.EncodeFilter
 import Bitmap.Lemmas.Png.DynamicEncoder
+import Bitmap.Lemmas.Png.Lz77
 import Bitmap.Lemmas.Png.DynamicEncoderDecode
 import Bitmap.Lemmas.Png.DynamicEncoderPayload
 import Bitmap.Lemmas.Png.FixedLiteral
